lunarlander/basic.thy
@@ -1,39 +1,44 @@
 theory basic
-   imports NthRoot  HHL_SL
+  imports HOL.NthRoot HHL_SL
 begin
 
+lemma real_val_simp: "(case Real x of Real c \<Rightarrow> A c | _ \<Rightarrow> X) = A x"
+  by (rule Syntax_SL.val.case(1))
+thm Syntax_SL.val.exhaust
 definition x :: exp where
-"x == RVar ''parx''"
+  "x == RVar ''parx''"
 
 
 definition Assignment :: proc where 
-"Assignment == x :=((Con Real 1) [+] x )"
+  "Assignment == x := ((Con Real 1) [+] x)"
 
-lemma B01:"{x[\<ge>](Con Real 0)}x :=((Con Real 1) [+] x ){x[\<ge>](Con Real 1);elE 0}"
+lemma B01:
+  "{x[\<ge>](Con Real 0)} x := ((Con Real 1) [+] x) {x[\<ge>](Con Real 1); elE 0}"
+  unfolding x_def
+  apply (rule AssignRRule, auto, fold x_def)
+proof -
+  fix s
+  assume a: "(x[\<ge>]Con Real 0) s"
+  obtain c where evalx: "evalE x s = Real c"
+    using a[unfolded fGreaterEqual_def]
+    apply (cases "evalE x s") by auto
+  show "(x[\<ge>]Con Real 1) (\<lambda>(y, i). if y = ''parx'' \<and> i = R then evalE (Con Real 1 [+] x) s else s (y, i))" 
+  proof -
+    have eval0: "evalE (Con Real 0) s = Real 0"
+      by auto
+    from a[unfolded fGreaterEqual_def] evalx eval0
+    have nonneg_c: "0 \<le> c" by auto
+    have evalx': "s (''parx'', R) = Real c"
+      using evalx unfolding x_def evalE.simps(2) by auto
+    show ?thesis
+      unfolding fGreaterEqual_def x_def evalE.simps(2) evalE.simps(1)
+      by (simp add: evalx' nonneg_c)
+  qed
+qed
 
-
-
-
-
-
-apply (cut_tac p="x[\<ge>](Con Real 0)" 
-           and q="x[\<ge>](Con Real 1)" 
-           and H="elE 0" 
-           and x="''parx''" 
-           and f="((Con Real 1) [+] x )" in  AssignRRule,auto)
-
-
-
-defer apply (simp add:x_def)
-apply (simp add:fGreaterEqual_def)
-apply (simp add:fNot_def)
-apply (simp add:fLess_def)
-apply (simp add:x_def)
-
-
-sorry
-lemma B02:"{x[\<ge>](Con Real 1)} (x :=((Con Real 1) [+] x ))*&& x[\<ge>](Con Real 1) {x[\<ge>](Con Real 1);elE 0}"
-apply (cut_tac Inv="x[\<ge>](Con Real 1)" 
+lemma B02:
+  "{x[\<ge>](Con Real 1)} (x :=((Con Real 1) [+] x ))*&& x[\<ge>](Con Real 1) {x[\<ge>](Con Real 1);elE 0}"
+apply (cut_tac I="x[\<ge>](Con Real 1)" 
            and P="x :=((Con Real 1) [+] x )" 
            and H="elE 0" 
             in  RepetitionRule,auto)
@@ -47,8 +52,6 @@ apply (cut_tac p="x[\<ge>](Con Real 1)"
            and f="((Con Real 1) [+] x )" in  AssignRRule,auto)
 defer apply (simp add:x_def)
 apply (simp add:fGreaterEqual_def)
-apply (simp add:fNot_def)
-apply (simp add:fLess_def)
 apply (simp add:x_def)
 sorry
 
